SATtypes.v
@@ -2,7 +2,6 @@
 Require Import ZF ZFpairs ZFsum ZFind_nat Sat.
 Require Import ZFlambda.
 Require Import Lambda.
-Module Lc:=Lambda.
 
 Set Implicit Arguments.
 
@@ -11,24 +10,47 @@ Set Implicit Arguments.
 Definition unitSAT :=
   interSAT (fun C => prodSAT C C).
 
-Definition ID := Lc.Abs (Lc.Ref 0).
+Definition ID := Abs (Ref 0).
 
 Lemma ID_intro : inSAT ID unitSAT.
 apply interSAT_intro with (1:=snSAT).
 intros.
 apply prodSAT_intro; intros.
-unfold Lc.subst; simpl Lc.subst_rec.
-rewrite Lc.lift0.
+unfold subst; simpl subst_rec.
+rewrite lift0.
 trivial.
 Qed.
 
 (** Disjoint sum *)
 
 Definition INL (t:term) :=
-  Lc.Abs (Lc.Abs (Lc.App (Lc.Ref 1) (Lc.lift 2 t))).
+  Abs (Abs (App (Ref 1) (lift 2 t))).
 Definition INR (t:term) :=
-  Lc.Abs (Lc.Abs (Lc.App (Lc.Ref 0) (Lc.lift 2 t))).
+  Abs (Abs (App (Ref 0) (lift 2 t))).
 
+Lemma INL_iota t1 t2 a :
+  redp (App2 (INL a) t1 t2) (App t1 a).
+unfold INL.
+eapply t_trans;[apply redp_app_l;apply t_step;apply red1_beta; reflexivity|].
+unfold subst; simpl.
+rewrite simpl_subst; trivial.
+apply t_step; apply red1_beta.
+unfold subst; simpl.
+repeat rewrite simpl_subst; trivial.
+repeat rewrite lift0; trivial.
+Qed.
+
+Lemma INR_iota t1 t2 a :
+  redp (App2 (INR a) t1 t2) (App t2 a).
+unfold INR.
+eapply t_trans;[apply redp_app_l;apply t_step;apply red1_beta; reflexivity|].
+unfold subst; simpl.
+rewrite simpl_subst; trivial.
+apply t_step; apply red1_beta.
+unfold subst; simpl.
+rewrite simpl_subst; trivial.
+repeat rewrite lift0; trivial.
+Qed.
 
 Definition sumReal (X Y:set->SAT) (a:set) : SAT :=
   interSAT (fun C =>
@@ -41,7 +63,7 @@ Lemma Real_sum_case X Y a RX RY C t b1 b2 :
   inSAT t (sumReal RX RY a) ->
   inSAT b1 (piSAT0 (fun x => a==inl x) RX (fun _ => C)) ->
   inSAT b2 (piSAT0 (fun x => a==inr x) RY (fun _ => C)) ->
-  inSAT (Lc.App2 t b1 b2) C.
+  inSAT (App2 t b1 b2) C.
 intros.
 apply interSAT_elim with (x:=C) in H0.
 eapply prodSAT_elim;[apply prodSAT_elim with (1:=H0)|]; trivial.
@@ -55,12 +77,12 @@ intros.
 apply interSAT_intro; auto.
 intros.
 apply prodSAT_intro; intros.
-unfold Lc.subst; simpl Lc.subst_rec.
-unfold Lc.subst; rewrite Lc.simpl_subst; auto.
+unfold subst; simpl subst_rec.
+unfold subst; rewrite simpl_subst; auto.
 apply prodSAT_intro; intros.
-unfold Lc.subst; simpl Lc.subst_rec.
-unfold Lc.subst; repeat rewrite Lc.simpl_subst; auto.
-repeat rewrite Lc.lift0.
+unfold subst; simpl subst_rec.
+unfold subst; repeat rewrite simpl_subst; auto.
+repeat rewrite lift0.
 apply piSAT0_elim with (x:=x) (u:=t) in H1; auto with *.
 Qed.
 
@@ -72,13 +94,192 @@ intros.
 apply interSAT_intro; auto.
 intros.
 apply prodSAT_intro; intros.
-unfold Lc.subst; simpl Lc.subst_rec.
-unfold Lc.subst; rewrite Lc.simpl_subst; auto.
+unfold subst; simpl subst_rec.
+unfold subst; rewrite simpl_subst; auto.
 apply prodSAT_intro; intros.
-unfold Lc.subst; simpl Lc.subst_rec.
-unfold Lc.subst; repeat rewrite Lc.simpl_subst; auto.
-repeat rewrite Lc.lift0.
+unfold subst; simpl subst_rec.
+unfold subst; repeat rewrite simpl_subst; auto.
+repeat rewrite lift0.
 apply piSAT0_elim with (x:=x) (u:=t) in H2; auto with *.
+Qed.
+
+(** Sigma-types *)
+
+Definition COUPLE t1 t2 :=
+  Abs (App2 (Ref 0) (lift 1 t1) (lift 1 t2)).
+
+Lemma COUPLE_iota t1 t2 b:
+  redp (App (COUPLE t1 t2) b) (App2 b t1 t2).
+unfold COUPLE.
+apply t_step; apply red1_beta.
+unfold subst; simpl.
+repeat rewrite simpl_subst; trivial.
+repeat rewrite lift0; trivial.
+Qed.
+
+Definition sigmaReal (X:set->SAT) (Y:set->set->SAT) (a:set) : SAT :=
+  interSAT (fun C => prodSAT (prodSAT (X (fst a)) (prodSAT (Y (fst a) (snd a)) C)) C).
+
+Lemma Real_couple x y X Y t1 t2 :
+  Proper (eq_set ==> eqSAT) X ->
+  Proper (eq_set ==> eq_set ==> eqSAT) Y ->
+  inSAT t1 (X x) ->
+  inSAT t2 (Y x y) ->
+  inSAT (COUPLE t1 t2) (sigmaReal X Y (couple x y)).
+intros.
+apply interSAT_intro; intros.
+ exact snSAT.
+apply prodSAT_intro; intros.
+unfold subst; simpl subst_rec.
+repeat rewrite simpl_subst; auto.
+repeat rewrite lift0.
+rewrite fst_def in H3.
+rewrite snd_def in H3.
+apply prodSAT_elim with (2:=H2).
+apply prodSAT_elim with (2:=H1); trivial.
+Qed.
+
+Lemma Real_sigma_elim X Y a C t b :
+  inSAT t (sigmaReal X Y a) ->
+  inSAT b (prodSAT (X (fst a)) (prodSAT (Y (fst a) (snd a)) C)) ->
+  inSAT (App t b) C.
+intros.
+apply interSAT_elim with (x:=C) in H.
+apply prodSAT_elim with (1:=H) (2:=H0).
+Qed.
+
+Lemma Real_sigma_elim' X Y RX RY a C t b :
+  ext_fun X Y ->
+  Proper (eq_set ==> eqSAT) C ->
+  a ∈ sigma X Y ->
+  inSAT t (sigmaReal RX RY a) ->
+  inSAT b (piSAT0 (fun x => x∈X) RX
+           (fun x => piSAT0 (fun y => y ∈ Y x) (RY x) (fun y => C(couple x y)))) ->
+  inSAT (App t b) (C a).
+intros.
+assert (eqa := surj_pair _ _ _ (subset_elim1 _ _ _ H1)).
+rewrite eqa.
+apply Real_sigma_elim with RX RY a; trivial.
+apply prodSAT_intro'; intros.
+apply prodSAT_intro'; intros.
+apply piSAT0_elim' in H3; red in H3.
+specialize H3 with (1:=fst_typ_sigma _ _ _ H1) (2:=H4).
+apply piSAT0_elim' in H3; red in H3.
+apply H3; trivial.
+apply snd_typ_sigma with (A:=X); auto with *.
+Qed.
+
+(** * Structural fixpoint. *)
+
+(** To avoid non-termination, we need to insert a "guard" operator G to control
+    the self-application of the fixpoint.
+ *)
+
+Definition FIXP G m :=
+  App G (Abs (App (lift 1 m) (App (lift 1 G) (Ref 0)))).
+
+(** when the guard expands when applied to n (e.g. when it's a constructor),
+    then the fixpoint unrolls once. *)
+Lemma FIXP_sim : forall G m n,
+  (forall m, redp (App2 G m n) (App2 m m n)) ->
+  redp (App (FIXP G m) n) (App2 m (FIXP G m) n).
+intros G m n Gsim.
+unfold FIXP at 1.
+eapply t_trans.
+ apply Gsim.
+apply redp_app_l.
+apply t_step.
+apply red1_beta.
+set (t1 := Abs (App (lift 1 m) (App (lift 1 G) (Ref 0)))).
+unfold subst; simpl.
+repeat rewrite simpl_subst; auto.
+repeat rewrite lift0.
+reflexivity.
+Qed.
+
+Lemma FIXP_sn G m:
+  (forall m, sn m -> sn (App G m)) ->
+  sn (App m (App G (Ref 0))) ->
+  sn (FIXP G m).
+intros snG satm.
+unfold FIXP.
+apply snG; trivial.
+apply sn_abs.
+apply sn_subst with (Ref 0).
+unfold subst; simpl.
+repeat rewrite simpl_subst; auto.
+repeat rewrite lift0; auto.
+Qed.
+
+Require Import ZFord.
+
+Lemma FIXP_sat : forall G o T RT m X,
+  isOrd o ->
+  (forall m, sn m -> sn (App G m)) ->
+  (forall o x t m (X:SAT), isOrd o -> x ∈ T o ->
+   inSAT t (RT o x) ->
+   inSAT (App2 m m t) X ->
+   inSAT (App2 G m t) X) ->
+  (forall y n, isOrd y -> y ⊆ o -> n ∈ T y -> exists2 y', y' ∈ y & n ∈ T (osucc y')) ->
+  (forall y y' n, isOrd y -> isOrd y' -> n ∈ T y -> y ⊆ y' -> y' ⊆ o ->
+   eqSAT (RT y n) (RT y' n)) ->
+
+  (forall y y' n, isOrd y -> isOrd y' -> y ⊆ y' -> y' ⊆ o -> n ∈ T y ->
+   inclSAT (X y n) (X y' n)) ->
+  inSAT m (piSAT0 (fun o' => o' ∈ osucc o) 
+             (fun o1 => piSAT0 (fun n => n ∈ T o1) (RT o1) (X o1))
+             (fun o1 => let o2 := osucc o1 in
+                        piSAT0 (fun n => n ∈ T o2) (RT o2) (X o2))) ->
+  inSAT (FIXP G m) (piSAT0 (fun n => n ∈ T o) (RT o) (X o)).
+intros G o T RT m X oo snG Gsat Tcont Rirrel Xmono msat.
+elim oo using isOrd_ind; intros.
+apply piSAT0_intro.
+ apply FIXP_sn; trivial.
+ apply piSAT0_elim' in msat; red in msat.
+ eapply sat_sn; apply msat with (x:=o).
+  apply lt_osucc; trivial.
+
+  apply piSAT0_intro; intros.
+   apply snG.
+   apply sn_var.
+
+   apply Gsat with (2:=H2); trivial.
+   eapply prodSAT_elim; [|eexact H3].
+   apply prodSAT_elim with snSAT;apply varSAT.
+
+intros x u xty0 ureal.
+destruct Tcont with (3:=xty0) as (z,?,?); trivial.
+specialize H1 with (1:=H2).
+assert (zo : isOrd z).
+ apply isOrd_inv with y; trivial.
+assert (osucc z ⊆ y).
+ red; intros.
+ apply isOrd_plump with z; trivial.
+  eauto using isOrd_inv.
+  apply olts_le; trivial.
+
+assert (ureal' : inSAT u (RT (osucc z) x)).
+ apply Rirrel with (3:=H3) (4:=H4); auto.
+unfold FIXP.
+apply Gsat with (2:=H3)(3:=ureal') (x:=x); auto.
+eapply inSAT_context; intros.
+ apply inSAT_exp.
+  left; simpl.
+  rewrite Bool.orb_true_r.
+  apply Bool.orb_true_r.
+
+  unfold subst; simpl subst_rec.
+  repeat rewrite simpl_subst; auto.
+  repeat rewrite lift0.
+  change (inSAT (App m (FIXP G m)) S).
+  eexact H5.
+apply Xmono with (osucc z); auto.
+assert (z ∈ osucc o).
+ apply isOrd_trans with o; auto.
+ apply H0; trivial.
+apply piSAT0_elim' in msat; red in msat.
+specialize msat with (1:=H5) (2:=H1).
+apply piSAT0_elim' in msat; red in msat; auto.
 Qed.
 
 
@@ -250,5 +451,37 @@ transitivity (tiSAT F A o x0).
  red; intros; apply isOrd_trans with o; auto.
 
  apply tiSAT_morph; auto with *.
+Qed.
+
+Lemma FIXP_TI_sat : forall G o F A m X,
+  Proper (incl_set ==> incl_set) F ->
+  Proper ((eq_set ==> eqSAT) ==> eq_set ==> eqSAT) A ->
+  (forall R R' o', isOrd o' -> o' ⊆ o -> (forall x x', x ∈ TI F o' -> x==x' -> eqSAT (R x) (R' x')) ->
+   forall x x', x ∈ TI F (osucc o') -> x==x' -> eqSAT (A R x) (A R' x')) ->
+  isOrd o ->
+  (forall m, sn m -> sn (App G m)) ->
+  (forall o x t m (X:SAT), isOrd o -> x ∈ TI F o ->
+   inSAT t (tiSAT F A o x) ->
+   inSAT (App2 m m t) X ->
+   inSAT (App2 G m t) X) ->
+  (forall y y' n, isOrd y -> isOrd y' -> y ⊆ y' -> y' ⊆ o -> n ∈ TI F y ->
+   inclSAT (X y n) (X y' n)) ->
+  inSAT m (piSAT0 (fun o' => o' ∈ osucc o) 
+             (fun o1 => piSAT0 (fun n => n ∈ TI F o1) (tiSAT F A o1) (X o1))
+             (fun o1 => let o2 := osucc o1 in
+                        piSAT0 (fun n => n ∈ TI F o2) (tiSAT F A o2) (X o2))) ->
+  inSAT (FIXP G m) (piSAT0 (fun n => n ∈ TI F o) (tiSAT F A o) (X o)).
+intros.
+apply FIXP_sat; trivial.
+ intros.
+ apply TI_elim in H9; auto.
+ destruct H9 as (o',?,?); exists o'; trivial.
+ rewrite TI_mono_succ; eauto using isOrd_inv.
+
+ intros.
+ apply tiSAT_mono; trivial.
+ intros.
+ apply H1 with (o':=o'); trivial.
+ transitivity y'; trivial.
 Qed.
 
